Matroid/Extremal/Thickness.lean
@@ -1,0 +1,38 @@
+import Matroid.Extremal.Covers
+
+set_option linter.style.longLine false
+
+variable {α : Type*} {M N M' : Matroid α} {I F X Y F' F₀ F₁ F₂ P L H H₁ H₂ H' B C D K : Set α}
+  {e f : α} {l r : ℕ} {a k : ℕ∞} {T : Set (Set α)} {ι : Type*} {i j : ι}
+  {P P' : Matroid α → Set α → Prop}
+
+open Set
+namespace Matroid
+
+section defs
+
+--Ask about -1. Do we need M.RankPos?
+
+def IsThick (M : Matroid α) (d : ℕ∞) : Prop := d ≤ M.coverNumber (fun M X ↦ M.eRk X ≤ (M.eRank - 1))
+
+def IsThick_set (M : Matroid α) (X : Set α ) (d : ℕ∞) : Prop :=
+    (M ↾ X).IsThick d
+
+lemma IsThick_set_iff (M : Matroid α) (X : Set α ) (d : ℕ∞) :
+    M.IsThick_set X d ↔ d ≤ (M ↾ X).coverNumber (fun M X ↦ M.eRk X ≤ (M.eRk X - 1)) := by
+  sorry
+
+lemma IsThick_two [M.Nonempty] (M : Matroid α) : M.IsThick 2 := by
+  obtain ht | ⟨T, hT, hTe ⟩ := exists_cover M (fun M X ↦ M.eRk X ≤ (M.eRank - 1))
+  · unfold IsThick
+    rw [ ht]
+    simp
+  unfold IsThick
+  rw [←hTe]
+  have : M.IsRankCover (M.eRank - 1) T := by sorry
+  --( IsRankCover_iff_IsCover M (M.eRank - 1) T ).2 hT
+  --IsRankCover_two
+  sorry
+
+
+end defs
